\section*{2.5 b}

\noindent
From 2.27 and part a, and $E(X) = 0$ and $X^{T} X \rightarrow N Cov(X)$, we 
have:

\begin{gather*}
\sigma^{2} + \sigma^{2} E_{x_{0}}[x_{0}^{T} (X^{T} X)^{-1} x_{0}]
\end{gather*}

\noindent
Consider $E_{x_{0}}[x_{0}^{T} (X^{T} X)^{-1} x_{0}]$. $x_{0}$ is a $p \times 1$ 
vector and $(X^{T} X)^{-1}$ will be $p \times p$, then 
$x_{0}^{T} (X^{T} X)^{-1} x_{0}$ is just a scalar. This means we can take the 
trace of this amount with out any consequence since it will just return itself. 
To motivate a maneuver we will use later in the proof, we will use 
$trace(A B) = trace(B A)$ with $A = x_{0}^{T} (X^{T} X)^{-1}$ and 
$B = x_{0}$.

\begin{gather*}
%--------------------------Line 1-----------------------------------------------
E_{x_{0}}[x_{0}^{T} (X^{T} X)^{-1} x_{0}] = 
E_{x_{0}}[trace(x_{0}^{T} (X^{T} X)^{-1} x_{0})] = \\
%--------------------------Line 2-----------------------------------------------
=
E_{x_{0}}[trace(x_{0} x_{0}^{T} (X^{T} X)^{-1})] = 
E_{x_{0}}[trace(x_{0} x_{0}^{T} \frac{(Cov(X))^{-1}}{N})] = \\
%--------------------------Line 3-----------------------------------------------
=
trace[E_{x_{0}}(x_{0} x_{0}^{T} \frac{(Cov(X))^{-1}}{N})] \\
%--------------------------Line 3-----------------------------------------------
\text{ since expectation and trace linear operators.}
\end{gather*}

\noindent
We now use the fact that $Cov(X)$ not depending on $x_{0}$ and 
$E_{x_{0}}(x_{0} x_{0}^{T} = Cov(x_{0}) = \sigma^{2}$. We also note that on our 
original assumption of the variance of $X$, $Cov(X) = \sigma^{2} \times I_{p} 
\implies (Cov(X))^{-1} = \frac{1}{\sigma^{2}} \times I_{p}$. Then we have: 

\begin{gather*}
%--------------------------Line 1-----------------------------------------------
trace[E_{x_{0}}(x_{0} x_{0}^{T} \frac{(Cov(X))^{-1}}{N})] = 
trace[\frac{(Cov(X))^{-1}}{N} E_{x_{0}}(x_{0} x_{0}^{T})] = \\
%--------------------------Line 2-----------------------------------------------
=
trace[\frac{1}{N \sigma^{2}} I_{p} Cov(x_{0})] = 
trace[\frac{1}{N \sigma^{2}} I_{p} \sigma^{2}] = 
trace[\frac{1}{N} I_{p}] = 
\frac{1}{N} trace[I_{p}] = 
\frac{p}{N}
\end{gather*}

\noindent
Now we substitute this result into our original equation:

\begin{gather*}
\sigma^{2} + \sigma^{2} E_{x_{0}}[x_{0}^{T} (X^{T} X)^{-1} x_{0}] = 
\sigma^{2} + \sigma^{2} \times \frac{p}{N} = 
\sigma^{2} \frac{p}{N} + \sigma^{2}
\end{gather*}